automat/CaseStudy/MediumSPS.thy
@@ -18,8 +18,8 @@ begin
 
 text {* @{term MedSPS}: Lossy medium function set for the Alternating Bit Protocol. *}
 definition MedSPS :: "nat \<Rightarrow> 'a medMessage tsyn SPS" where 
-  "MedSPS n = Abs_uspec (Rev {(MedSPF ora) | ora. ora \<in> (oraFun n)}, Discr {\<C> ''ds''}, 
-  Discr {\<C> ''dr''})"
+  "MedSPS n = Abs_uspec (Rev {(MedSPF ora) | ora. ora \<in> (oraFun n)}, Discr medInDom, 
+  Discr medOutDom)"
 
 (* ----------------------------------------------------------------------- *)
 subsection {* Basic Properties of MedSPS *}
@@ -28,7 +28,7 @@ subsection {* Basic Properties of MedSPS *}
 text{* @{term MedSPS} is well-formed. *}
 lemma medsps_uspecwell [simp]: 
   "uspecWell (Rev {(MedSPF ora) | ora. (#({True} \<ominus> ora) = \<infinity> \<and> snth n ora
-   \<and> (\<forall>k<n. \<not>snth k ora))}) (Discr {\<C> ''ds''}) (Discr {\<C> ''dr''})"
+   \<and> (\<forall>k<n. \<not>snth k ora))}) (Discr medInDom) (Discr medOutDom)"
   apply (rule uspec_wellI)
   apply (simp add: ufclDom_ufun_def)
   using medspf_ufdom apply blast
@@ -36,14 +36,16 @@ lemma medsps_uspecwell [simp]:
   using medspf_ufran by blast
 
 text{* The domain of @{term MedSPS}. *}
-lemma medsps_uspecdom: "uspecDom\<cdot>(MedSPS n) = {\<C> ''ds''}"
-  using medsps_uspecwell
-  by (simp add: MedSPS_def uspecdom_insert oraFun_def)
+lemma medsps_uspecdom: "uspecDom\<cdot>(MedSPS n) = medInDom"
+  using medsps_uspecwell  
+  apply (simp add: MedSPS_def uspecdom_insert oraFun_def)
+sorry
 
 text{* The range of @{term MedSPS}. *}
-lemma medsps_uspecran: "uspecRan\<cdot>(MedSPS n) = {\<C> ''dr''}"
+lemma medsps_uspecran: "uspecRan\<cdot>(MedSPS n) = medOutDom"
   using medsps_uspecwell 
-  by (simp add: MedSPS_def uspecran_insert oraFun_def)
+  apply (simp add: MedSPS_def uspecran_insert oraFun_def)
+sorry
 
 (* ----------------------------------------------------------------------- *)
 subsection {* Medium State Lemmata *}
@@ -59,29 +61,28 @@ lemma slen_createbundle_getch: "#(createBundle (\<M> m) c  .  c) < \<infinity>"
     lscons_conv option.sel order_less_le slen_scons strict_slen sup'_def ubabs_ubrep)
 
 lemma medsps_0_uspecwell: 
-  "uspecWell (Rev{MedSPF ora |ora::bool stream. #({True} \<ominus> ora) = \<infinity> \<and> shd ora}) (Discr{\<C> ''ds''}) 
-  (Discr{\<C> ''dr''})"
-  using medsps_uspecwell
+  "uspecWell (Rev{MedSPF ora |ora::bool stream. #({True} \<ominus> ora) = \<infinity> \<and> shd ora}) (Discr medInDom) 
+  (Discr medOutDom)"
   proof -
     have "{MedSPF ora |ora::bool stream. #({True} \<ominus> ora) = \<infinity> \<and> shd ora} 
       = {(MedSPF ora) | ora. (#({True} \<ominus> ora) = \<infinity> \<and> snth 0 ora \<and> (\<forall>k<0. \<not>snth k ora))}"
-    by simp
+      by simp
     then show ?thesis
-    using medsps_uspecwell by presburger
+      using medsps_uspecwell by presburger
   qed
 
 (* If a "null" comes in, send it out and stay in the same state. *)
 lemma "spsConcIn (tsynbNull(\<C> ''ds'')) (MedSPS n) = spsConcOut (tsynbNull (\<C> ''dr''))\<cdot>(MedSPS n)"
-  apply (subst spsconcin_insert)
+ (* apply (subst spsconcin_insert)
   apply (case_tac "c=(\<C> ''dr'')", simp_all)
   apply (subst spsconcout_insert, simp)
   apply (simp add: spfConcIn_def spfConcOut_def)
-  apply (simp add: uspecImage_def medsps_uspecran medsps_uspecdom ufclDom_ufun_def ufclRan_ufun_def)
+  apply (simp add: uspecImage_def medsps_uspecran medsps_uspecdom ufclDom_ufun_def ufclRan_ufun_def)*)
 sorry
 
 lemma "spsConcIn (createBundle (Msg m) (\<C> ''ds'')) (MedSPS (Suc n))
   = spsConcOut (tsynbNull(\<C> ''dr''))\<cdot>(MedSPS n)"
-  apply (subst spsconcin_insert)
+(*  apply (subst spsconcin_insert)
   apply (case_tac "c=(\<C> ''dr'')", simp_all)
   apply (simp add: slen_createbundle_getch)
   apply (subst spsconcout_insert, simp)
@@ -90,10 +91,10 @@ lemma "spsConcIn (createBundle (Msg m) (\<C> ''ds'')) (MedSPS (Suc n))
   apply (simp add: uspecrevset_insert MedSPS_def)
   using medsps_uspecwell
   apply (simp add: setrevImage_def inv_rev_rev)
-  apply (simp add: MedSPF_def)
+  apply (simp add: MedSPF_def)*)
 sorry
 
-lemma "\<And>x::(abpMessage tsyn stream\<^sup>\<Omega>) ufun.
+(*lemma "\<And>x::(abpMessage tsyn stream\<^sup>\<Omega>) ufun.
        (x \<in> Rep_cfun (spfConcIn (createBundle (\<M> m) (\<C> ''ds''))) ` Rep_rev_uspec (MedSPS (0::nat))) =
        (x \<in> Rep_cfun (spfConcOut (createBundle (\<M> m) (\<C> ''dr''))) ` Rep_rev_uspec (MedSPS n))"
   apply (simp add: image_def spfConcIn_def spfConcOut_def)
@@ -104,11 +105,11 @@ lemma "\<And>x::(abpMessage tsyn stream\<^sup>\<Omega>) ufun.
   apply (smt CollectD medspf_ufdom medspf_ufran ufclDom_ufun_def ufclRan_ufun_def uspec_wellI)
   proof -
     obtain xa where "xa \<in> {MedSPF ora |ora. #({True} \<ominus> ora) = \<infinity> \<and> shd ora}"    
-  oops
+  oops*)
 
 lemma "spsConcIn (createBundle (Msg m) (\<C> ''ds'')) (MedSPS 0) 
   = spsConcOut (createBundle (Msg m) (\<C> ''dr''))\<cdot>(MedSPS n)"
-  apply (subst spsconcin_insert)
+(*  apply (subst spsconcin_insert)
   apply (simp add: slen_createbundle_getch)
   apply (subst spsconcout_insert)
   apply (simp add: slen_createbundle_getch)
@@ -126,23 +127,7 @@ lemma "spsConcIn (createBundle (Msg m) (\<C> ''ds'')) (MedSPS 0)
   defer
   apply (subst rep_abs_rev_simp)
   defer
-  apply (simp add: set_eq_iff)
+  apply (simp add: set_eq_iff)*)
 sorry
-
-(*
-apply (rule set_eq_iff)
-
-(* If a "null" comes in send it out and stay in the same state *) 
-lemma "spsConcIn (makeNull (\<C> ''ds'')) (h_MED state) = spsConcOut (makeNull (\<C> ''dr''))\<cdot>(h_MED state)"
-  oops
-
-(* counter not null, drop every message and count one down *)
-lemma "spsConcIn (makeInput m) (h_MED (State TheOne (Suc n))) = spsConcOut (makeNull (\<C> ''dr''))\<cdot>(h_MED (State TheOne n))"
-  oops
-
-(* Counter hit zero, so pass the message and reset the countdown to a random value *)
-lemma "spsConcIn (makeInput m) (h_MED (State TheOne 0)) = spsConcOut (makeOutput m)\<cdot>(spsFlatten {h_MED (State TheOne n) |  n. True})"
-  oops
-*)
 
 end
